Update translator proofs

coq/FSigmaHCOL/FHCOLtoLFHCOL.v
@@ -1,4 +1,5 @@
 Require Import Helix.Tactics.StructTactics.
+Require Import Helix.Util.OptionSetoid.
 
 Require Import Helix.FSigmaHCOL.Float64asCT.
 Require Import Helix.FSigmaHCOL.LazyFloat64asCT.
@@ -8,6 +9,8 @@ Require Import Helix.DSigmaHCOL.DHCOLTypeTranslator.
 
 Require Import MathClasses.interfaces.canonical_names.
 Require Import ZArith String Psatz.
+
+Require Import ExtLib.Structures.Monad.
 
 Module Export FHCOLtoLFHCOL := MDHCOLTypeTranslator
                                  (MFloat64asCT)
@@ -19,27 +22,148 @@ Module Export FHCOLtoLFHCOL := MDHCOLTypeTranslator
                                  (FHCOLEval)
                                  (LFHCOLEval).
 
+Inductive heq_Float_SymFloat : MFloat64asCT.t -> MLazyFloat64asCT.t -> Prop :=
+| heq_FSF_Some : forall f sf,
+    evalSymFloat sf ≡ Some f -> heq_Float_SymFloat f sf
+| heq_FSF_None : forall f, heq_Float_SymFloat f None.
+
 Global Instance FLF_CHE : FHCOLtoLFHCOL.CTranslation_heq.
 Proof.
   econstructor.
   -
-    instantiate (1:=fun f lf => f = evalFloatExpr lf).
+    instantiate (1:=heq_Float_SymFloat).
     intros f1 f2 F lf1 lf2 LF.
-    rewrite F, LF.
+    invc F; invc LF.
     easy.
   -
     intros * T.
     unfold translateCTypeConst in *.
-    repeat break_if; invc T;
-      now rewrite e, <-H1.
+    repeat break_if; invc T.
+    all: rewrite e.
+    all: constructor.
+    all: now rewrite <-H1.
 Defined.
 
 Global Instance FLF_COP : @FHCOLtoLFHCOL.COpTranslationProps FLF_CHE.
 Proof.
-  do 2 constructor; intros.
-  all: unfold heq_CType, FLF_CHE in *.
-  all: cbn.
-  all: congruence.
+  do 2 constructor.
+  all: intros * XE; try intro YE.
+  -
+    inversion XE as [t1 t2 EX t3 t4| t1 t2 EX]; clear XE; subst;
+      inversion YE as [t1 t2 EY t3 t4| t1 t2 EY]; clear YE; subst.
+    2-4: cbn; repeat break_match; constructor 2.
+    destruct x' as [[xe xf] |],
+             y' as [[ye yf] |]; try some_none.
+    all: cbn in *.
+    2-4: constructor 2.
+    all: destruct (List.list_eq_dec MFloat64asCT.CTypeEquivDec xe ye)
+      as [EEQ | ENEQ].
+    all: repeat break_match; subst.
+    6: constructor 2.
+    all: constructor; cbn.
+    all: rewrite ?EX, ?EY.
+    all: try erewrite evalFloatExpr_env_indep by eassumption.
+    all: try reflexivity.
+    now rewrite EEQ, EY.
+  -
+    inversion XE as [t1 t2 EX t3 t4| t1 t2 EX]; clear XE; subst;
+      inversion YE as [t1 t2 EY t3 t4| t1 t2 EY]; clear YE; subst.
+    2-4: cbn; repeat break_match; constructor 2.
+    destruct x' as [[xe xf] |],
+             y' as [[ye yf] |]; try some_none.
+    all: cbn in *.
+    2-4: constructor 2.
+    all: destruct (List.list_eq_dec MFloat64asCT.CTypeEquivDec xe ye)
+      as [EEQ | ENEQ].
+    all: repeat break_match; subst.
+    6: constructor 2.
+    all: constructor; cbn.
+    all: rewrite ?EX, ?EY.
+    all: try erewrite evalFloatExpr_env_indep by eassumption.
+    all: try reflexivity.
+    now rewrite EEQ, EY.
+  -
+    inversion XE as [t1 t2 EX t3 t4| t1 t2 EX]; clear XE; subst;
+      inversion YE as [t1 t2 EY t3 t4| t1 t2 EY]; clear YE; subst.
+    2-4: cbn; repeat break_match; constructor 2.
+    destruct x' as [[xe xf] |],
+             y' as [[ye yf] |]; try some_none.
+    all: cbn in *.
+    2-4: constructor 2.
+    all: destruct (List.list_eq_dec MFloat64asCT.CTypeEquivDec xe ye)
+      as [EEQ | ENEQ].
+    all: repeat break_match; subst.
+    6: constructor 2.
+    all: constructor; cbn.
+    all: rewrite ?EX, ?EY.
+    all: try erewrite evalFloatExpr_env_indep by eassumption.
+    all: try reflexivity.
+    now rewrite EEQ, EY.
+  -
+    inversion XE as [t1 t2 EX t3 t4| t1 t2 EX]; clear XE; subst;
+      inversion YE as [t1 t2 EY t3 t4| t1 t2 EY]; clear YE; subst.
+    2-4: cbn; repeat break_match; constructor 2.
+    destruct x' as [[xe xf] |],
+             y' as [[ye yf] |]; try some_none.
+    all: cbn in *.
+    2-4: constructor 2.
+    all: destruct (List.list_eq_dec MFloat64asCT.CTypeEquivDec xe ye)
+      as [EEQ | ENEQ].
+    all: repeat break_match; subst.
+    6: constructor 2.
+    all: constructor; cbn.
+    all: rewrite ?EX, ?EY.
+    all: try erewrite evalFloatExpr_env_indep by eassumption.
+    all: try reflexivity.
+    now rewrite EEQ, EY.
+  -
+    inversion XE as [t1 t2 EX t3 t4| t1 t2 EX]; clear XE; subst;
+      inversion YE as [t1 t2 EY t3 t4| t1 t2 EY]; clear YE; subst.
+    2-4: cbn; repeat break_match; constructor 2.
+    destruct x' as [[xe xf] |],
+             y' as [[ye yf] |]; try some_none.
+    all: cbn in *.
+    2-4: constructor 2.
+    all: destruct (List.list_eq_dec MFloat64asCT.CTypeEquivDec xe ye)
+      as [EEQ | ENEQ].
+    all: repeat break_match; subst.
+    6: constructor 2.
+    all: constructor; cbn.
+    all: rewrite ?EX, ?EY.
+    all: try erewrite evalFloatExpr_env_indep by eassumption.
+    all: try reflexivity.
+    now rewrite EEQ, EY.
+  -
+    inversion XE as [t1 t2 EX t3 t4| t1 t2 EX]; clear XE; subst;
+      inversion YE as [t1 t2 EY t3 t4| t1 t2 EY]; clear YE; subst.
+    2-4: cbn; repeat break_match; constructor 2.
+    destruct x' as [[xe xf] |],
+             y' as [[ye yf] |]; try some_none.
+    all: cbn in *.
+    2-4: constructor 2.
+    all: destruct (List.list_eq_dec MFloat64asCT.CTypeEquivDec xe ye)
+      as [EEQ | ENEQ].
+    all: repeat break_match; subst.
+    6: constructor 2.
+    all: constructor; cbn.
+    all: rewrite ?EX, ?EY.
+    all: try erewrite evalFloatExpr_env_indep by eassumption.
+    all: try reflexivity.
+    now rewrite EEQ, EY.
+  -
+    inversion XE as [t1 t2 EX t3 t4| t1 t2 EX]; clear XE; subst.
+    2: constructor 2.
+    destruct x' as [[xe xf] |]; try some_none.
+    2: constructor 2.
+    constructor; cbn in *.
+    now rewrite EX.
+  -
+    inversion XE as [t1 t2 EX t3 t4| t1 t2 EX]; clear XE; subst.
+    2: constructor 2.
+    destruct x' as [[xe xf] |]; try some_none.
+    2: constructor 2.
+    constructor; cbn in *.
+    now rewrite EX.
 Qed.
 
 (* Trivial instances for "translating" Int64 -> Int64 *)
